Java/src/Logic/AssertionLogic.v
@@ -3,10 +3,14 @@
    make this easier. Ideally, this file should not be larger than a few tens of lines
    at most. *)
 
-Require Import ILogic ILInsts SepAlg SepAlgPfun BILogic BILInsts IBILogic SepAlgMap Maps String Rel.
+Add Rec LoadPath "/Users/jebe/git/Charge/Charge!/bin".
+Add Rec LoadPath "/Users/jebe/git/Java/Java/bin".
+
+Require Import ILogic ILInsts SepAlg BILogic BILInsts IBILogic SepAlgMap Maps String Rel.
 Require Import RelationClasses Setoid Morphisms Program. 
 Require Import MapInterface MapFacts.
 Require Import Open Stack Lang OpenILogic Pure ILEmbed.
+Require Import UUSepAlg SepAlgInsts HeapArr.
 
 Local Existing Instance ILPre_Ops.
 Local Existing Instance ILPre_ILogic.
@@ -24,15 +28,32 @@ Local Existing Instance MapSepAlgOps.
 Local Existing Instance MapSepAlg.
 Local Existing Instance MapEquiv.
 Local Existing Instance EquivPreorder.
+Local Existing Instance UUMapSepAlg.
+Local Existing Instance SepAlgOps_prod.
+Local Existing Instance SepAlg_prod.
+Local Existing Instance UUSepAlg_prod.
 
-Definition heap := Map [ptr * field, val].
+Definition heap_ptr := Map [ptr * field, val].
 
-Definition heap_unit : heap := @map_unit _ _ _ val.
+Definition heap := (heap_ptr * heap_arr)%type.
+
+Definition heap_ptr_unit : heap_ptr := @map_unit _ _ _ val.
+Definition heap_unit : heap := (heap_ptr_unit, heap_arr_unit).
+
+Definition heap_add_ptr (h : heap) (p : ptr) (f : field) (v : val) : heap :=
+  (add (p, f) v (fst h), snd h).
+Definition heap_add_arr (h : heap) (n m : nat) (v : val) : heap :=
+  (fst h, add (n, m) v (snd h)).
+
+Instance RelHeapPtr : Rel heap_ptr := _.
+Instance PreorderHeapPtr : PreOrder (@rel heap_ptr RelHeapPtr) := _.
+Instance HeapPtrSepAlgOps : SepAlgOps heap_ptr := _.
+Instance SepAlgHeapPtr : UUSepAlg heap_ptr := _.
 
 Instance RelHeap : Rel heap := _.
 Instance PreorderHeap : PreOrder (@rel heap RelHeap) := _.
 Instance HeapSepAlgOps : SepAlgOps heap := _.
-Instance SepAlgHeap : SepAlg heap := _.
+Instance SepAlgHeap : UUSepAlg heap := _.
 
 Definition asn1 := ILPreFrm (@rel heap subheap) Prop.
 Instance ILogicOpsAsn1 : ILogicOps asn1 := _.
@@ -112,7 +133,6 @@ Instance PureSpec1 (S : spec1) : @Pure asn2 ILogicOpsAsn2 BILOperatorsAsn2 (embe
 Instance PureSpecAsn (S : spec) : @Pure asn _ _ (embed S) := _.
 Instance PureSpec (S : spec) : @Pure sasn _ _ (embed S) := _.
 
-
 Local Transparent ILPre_Ops.
 
 Definition mk_asn (f: Prog_wf -> nat -> heap -> Prop)
@@ -133,10 +153,341 @@ Grab Existential Variables.
 Defined.
 
 Program Definition pointsto_aux (x : ptr) (f : field) (v : val) : asn :=
-  mk_asn (fun P k h => subheap ((empty val) [(x, f) <- v]) h) _ _ _.
+  mk_asn (fun P k h => subheap ((empty val) [(x, f) <- v]) (fst h)) _ _ _.
 Next Obligation.
+  destruct h, h'; simpl in *.
+  apply subheap_prod in H as [H _].
   setoid_rewrite H in H0. assumption.
 Qed.
 
-Program Definition pointsto (p : val) (f : field) (v : val) : asn :=
+Definition pointsto (p : val) (f : field) (v : val) : asn :=
   (p <> null) /\\ pointsto_aux (val_to_ptr p) f v.
+
+Program Definition pointsto_arr_element_aux (x : val) (path : list val) (v : val) : asn :=
+  mk_asn (fun P k h => exists (h' : heap) , 
+                         subheap h' h /\
+                         find_heap_arr (val_to_nat x)
+                                       (List.map val_to_nat path) (snd h') = 
+                         Some v) _ _ _.
+Next Obligation.
+  exists H; split; [assumption | reflexivity].
+Qed.
+Next Obligation.
+  exists H0; split; [assumption | reflexivity].
+Qed.
+Next Obligation.
+  exists H0; split; [etransitivity; eassumption | reflexivity].
+Qed.
+
+Definition pointsto_arr_element (x i : val) (v : val) : asn := 
+  pointsto_arr_element_aux x (i::nil) v.
+
+Require Import ZArith.
+
+Fixpoint pointsto_arr_aux (x : val) (n : nat) (vs : list val) : asn :=
+  match vs with
+    | nil   => empSP
+    | v::vs => pointsto_arr_element x (vint (Z_of_nat n)) v ** 
+                                    pointsto_arr_aux x (S n) vs
+  end.
+
+Opaque ILogicOpsAsn.
+
+Lemma firstn_nil {A : Type} (n : nat) : firstn n (@nil A) = nil.
+Proof.
+  destruct n; simpl; reflexivity.
+Qed.
+
+Lemma skipn_nil {A : Type} (n : nat) : skipn n (@nil A) = nil.
+Proof.
+  destruct n; simpl; reflexivity.
+Qed.
+
+Lemma firstn_cons {A : Type} (n : nat) (x : A) (xs : list A) (H : n > 0) :
+  firstn n (x :: xs) = x :: (firstn (n - 1) xs).
+Proof.
+  destruct n; simpl.
+  + omega.
+  + replace (n - 0) with n by omega; reflexivity.
+Qed.
+
+Lemma firstn_app1 {A : Type} (n : nat) (xs ys : list A) (H : n <= List.length xs) :
+  firstn n (xs ++ ys) = firstn n xs.
+Proof.
+  generalize dependent n; induction xs; simpl in *; intros.
+  + assert (n = 0) by omega; clear H; subst; simpl; reflexivity.
+  + destruct n; simpl in *; [reflexivity|].
+    f_equal. apply IHxs. omega.
+Qed.
+  
+Lemma firstn_app2 {A : Type} (n : nat) (xs ys : list A) (H : n >= List.length xs) :
+  firstn n (xs ++ ys) = xs++(firstn (n - List.length xs) ys).
+Proof.
+  generalize dependent n; induction xs; simpl in *; intros.
+  + replace (n - 0) with n by omega; reflexivity.
+  + destruct n; simpl in *; [omega|].
+    f_equal. apply IHxs. omega.
+Qed.
+  
+Lemma skipn_cons {A : Type} (n : nat) (x : A) (xs : list A) (H : n > 0) :
+  skipn n (x :: xs) = skipn (n - 1) xs.
+Proof.
+  destruct n; simpl.
+  + omega.
+  + replace (n - 0) with n by omega; reflexivity.
+Qed.
+
+Lemma skipn_drop {A : Type} (n : nat) (xs : list A) (H : n >= List.length xs) :
+  skipn n xs = nil.
+Proof.
+  generalize dependent xs; induction n; simpl; intros.
+  + destruct xs; simpl in *; [reflexivity | omega].
+  + destruct xs; [reflexivity|].
+    apply IHn; simpl in *; omega.
+Qed.
+
+Lemma skipn_length {A : Type} (n : nat) (vs : list A) :
+  List.length (skipn n vs) = (List.length vs - n).
+Proof.
+  generalize dependent n; induction vs; simpl.
+  + destruct n; simpl; reflexivity.
+  + destruct n; simpl; [reflexivity|].
+    rewrite IHvs. reflexivity.
+Qed.
+      
+
+
+Lemma pointsto_arr_aux_app (x : val) (n : nat) (xs ys : list val) :
+  pointsto_arr_aux x n (xs++ys) -|- pointsto_arr_aux x n xs ** pointsto_arr_aux x (n + List.length xs) ys.
+Proof.
+  generalize dependent n; induction xs; simpl in *; intros.
+  + rewrite sepSPC, empSPR. replace (n + 0) with n by omega. reflexivity.
+  + rewrite IHxs. 
+    replace (n + S (Datatypes.length xs)) with (S n + Datatypes.length xs) by omega.
+    rewrite sepSPA. reflexivity.
+Qed.
+
+Lemma pointsto_arr_aux_split (x : val) (n m : nat) (vs : list val) (H : n < m) :
+  pointsto_arr_aux x n vs -|- pointsto_arr_aux x n (firstn (m - n) vs) **
+                              pointsto_arr_aux x m (skipn (m - n) vs).
+Proof.
+  rewrite <- (firstn_skipn (m - n) vs) at 1.
+  rewrite pointsto_arr_aux_app.
+  rewrite firstn_length.
+  destruct (Min.min_dec (m - n) (Datatypes.length vs)) as [H1 | H1]; rewrite H1.
+  + replace (n + (m - n)) with m by omega; reflexivity.
+  + rewrite skipn_drop; simpl; [reflexivity|].
+    setoid_rewrite <- H1.
+    assert (min (m - n) (Datatypes.length vs) <= m - n); [|omega].
+    apply Min.le_min_l.
+Qed.
+
+Definition pointsto_arr (x n m : val) (vs : list val) : asn :=
+  let n' := val_to_nat n in
+  let m' := val_to_nat m in
+  (n' <= m' /\ List.length vs = S (m' - n')) /\\ pointsto_arr_aux x n' vs.
+
+(* Gregory should be able to pull this off with his cancellation magic. *)
+
+Lemma embed_and_admit (p q : asn) (P Q : Prop) : 
+  (P /\\ p) ** (Q /\\ q) -|- P /\\ Q /\\ p ** q.
+Proof.
+  admit.
+Qed.
+
+
+Lemma pointsto_arr_split (x i j k : val) (vs : list val) 
+      (Hij : val_to_nat i <= val_to_nat j) 
+      (Hjk : val_to_nat j < val_to_nat k) :
+  pointsto_arr x i k vs -|- pointsto_arr x i j (firstn (S ((val_to_nat j) - 
+                                                           (val_to_nat i))) vs) ** 
+                            pointsto_arr x (vint (Z_of_nat (S (val_to_nat j)))) k 
+                                         (skipn (S ((val_to_nat j) - (val_to_nat i))) vs).
+Proof.
+  unfold pointsto_arr.
+   replace (val_to_nat (Z.of_nat (S (val_to_nat j)))) with (S (val_to_nat j)) by
+    (destruct j; unfold val_to_nat; simpl in *; try reflexivity;
+     rewrite SuccNat2Pos.id_succ; reflexivity).
+   split.
+  + apply lpropandL; intros [H1 H2].
+    rewrite embed_and_admit.
+    apply lpropandR. {
+      split; [assumption|].
+      rewrite firstn_length.
+      simpl. setoid_rewrite H2.
+      f_equal; apply Min.min_l; omega.
+    }
+    apply lpropandR. {
+      split; [omega|].
+      rewrite skipn_length; omega.
+    }
+    rewrite (pointsto_arr_aux_split x (val_to_nat i) (S(val_to_nat j))); [|omega].
+    replace (S (val_to_nat j) - val_to_nat i) with (S (val_to_nat j - val_to_nat i)) by omega.
+    reflexivity.
+
+  + rewrite embed_and_admit.
+    apply lpropandL; intros [H1 H2].
+    apply lpropandL; intros [H3 H4].
+    apply lpropandR. split; [omega|].
+    rewrite <- (firstn_skipn (S (val_to_nat j - val_to_nat i)) vs), app_length; omega.
+    etransitivity; [|rewrite (pointsto_arr_aux_split x (val_to_nat i) (S(val_to_nat j))); [|omega]]; [|reflexivity]. 
+    replace (S (val_to_nat j) - val_to_nat i) with (S (val_to_nat j - val_to_nat i)) by omega.
+    reflexivity.
+Qed.
+
+Transparent ILogicOpsAsn.
+Transparent BILOperatorsAsn.
+Transparent BILPre_Ops.
+Transparent EmbedAsnPropOp.
+Transparent EmbedILPreDropOpNeq.
+Transparent EmbedILPreDropOpEq.
+Opaque MapSepAlgOps.
+Opaque SepAlgOps_prod.
+
+Lemma pointsto_arr_pointsto_element_lst (x i : val) (vs : list val) :
+  pointsto_arr x i i vs |-- Exists v, vs = v::nil /\\ pointsto_arr_element x i v.
+Proof.
+  unfold pointsto_arr, pointsto_arr_element.
+  apply lpropandL; intros [H1 H2].
+  destruct vs; simpl in H2; [omega|].
+  destruct vs; simpl in H2; [|omega].
+  cbv [pointsto_arr_aux].
+  rewrite empSPR.
+  intros P n h H.
+  simpl in *.
+  destruct H as [h' [Hh H]].
+  exists v; split; simpl; [reflexivity|].
+  exists h'; split; [assumption|].
+  destruct h'; simpl in *.
+  assert (val_to_nat (Z.of_nat (val_to_nat i)) = val_to_nat i). {
+      clear H.
+      induction i; simpl in *; unfold val_to_nat in *; simpl in *; try reflexivity.
+      rewrite Nat2Z.id; reflexivity.
+    }
+  rewrite <- H0. apply H.
+Qed.
+
+Lemma pointsto_arr_pointsto_element (x i : val) (v : val) :
+  pointsto_arr x i i (v::nil) -|- pointsto_arr_element x i v.
+Proof.
+  split.
+  + rewrite pointsto_arr_pointsto_element_lst.
+    apply lexistsL; intro v'.
+    apply lpropandL; intros H; inversion H; subst; clear H.
+    reflexivity.
+  + unfold pointsto_arr_element, pointsto_arr.
+    apply lpropandR; [split; [reflexivity | simpl; omega]|].
+    cbv [pointsto_arr_aux]. rewrite empSPR.
+    intros P n h H; simpl in *.
+    destruct H as [h' [Hh H]].
+    exists h'; split; [apply Hh|].
+    assert (val_to_nat (Z.of_nat (val_to_nat i)) = val_to_nat i). {
+      clear H.
+      induction i; simpl in *; unfold val_to_nat in *; simpl in *; try reflexivity.
+      rewrite Nat2Z.id; reflexivity.
+    }
+    rewrite H0. apply H.
+Qed.
+
+Definition update {A : Type} (lst : list A) (n : nat) (p : A) :=
+  firstn n lst ++ (p::(skipn (n+1) lst)).
+(*
+Lemma pointsto_arr_update (x i j k : val) (vs : list val) (v : val) 
+      (Hij : val_to_nat i <= val_to_nat j) 
+      (Hjk : val_to_nat j < val_to_nat k) :
+  pointsto_arr x i k (update vs (val_to_nat j - val_to_nat i) v) -|- 
+  pointsto_arr x i j (firstn ((val_to_nat j) - 
+                              (val_to_nat i)) vs) ** 
+  pointsto_arr_element k j v **
+  pointsto_arr x (vint (Z_of_nat (S (val_to_nat j)))) k 
+  (skipn (S ((val_to_nat j) - (val_to_nat i))) vs).
+Proof.
+  rewrite pointsto_arr_split with (j := S (val_to_nat j)). try eassumption.
+  unfold update.
+  replace (firstn (val_to_nat j - val_to_nat i) vs ++
+                  v :: skipn (val_to_nat j - val_to_nat i + 1) vs) with
+  ((firstn (val_to_nat j - val_to_nat i) vs ++
+         (v::nil)) ++ (skipn (val_to_nat j - val_to_nat i + 1) vs)) 
+    by (rewrite <- app_assoc; reflexivity).
+  rewrite firstn_app1.
+  rewrite firstn_app2.
+  replace (S (val_to_nat j - val_to_nat i) -
+         Datatypes.length (firstn (val_to_nat j - val_to_nat i) vs)) with 1.
+  replace (firstn 1 (v :: nil)) with (v :: nil) by reflexivity.
+  cbv delta [firstn].
+SearchAbout firstn.
+  simpl.
+Qed.
+*)
+(*
+
+Lemma pointsto_arr_get_element x i j k vs
+      (Hij : val_to_nat i <= val_to_nat j)
+      (Hjk : val_to_nat j <= val_to_nat k) :
+      pointsto_arr x i k vs |-- pointsto_arr_element x j 
+                                (List.nth (val_to_nat j - val_to_nat i) vs null).
+Proof.
+  unfold pointsto_arr.
+  apply lpropandL; intros [H1 H2].
+  unfold pointsto_arr_element.
+  intros p n h; simpl; intros.
+  generalize dependent (val_to_nat i).
+  generalize dependent (val_to_nat j).
+  generalize dependent (val_to_nat k).
+  clear i j k.
+  intros k j Hjk i Hij Hik Hlength H.
+  destruct h as [hp ha].
+  exists (hp, heap_arr_unit [(val_to_nat x, j) <- nth (j - i) vs null]).
+  split; simpl; [|rewrite add_eq_o; reflexivity].
+  apply subheap_prod; split; [reflexivity|].
+  generalize dependent k; induction vs; simpl in *; intros. omega.
+  inversion Hlength; clear Hlength.
+  unfold sepSP in H. unfold BILOperatorsAsn in H.
+  simpl in H.
+  destruct H as [h1 [h2 [Hh [[h3 [H2 H3]] H4]]]].
+  destruct h1, h2, h3.
+  apply subheap_prod in H2 as [H2 H5].
+  simpl in *.
+  remember (j - i) as l; destruct l; simpl in *.
+  assert (i = j) by omega; subst.
+  admit.
+  admit.
+Qed.
+
+
+Fixpoint arr_heap (h : heap_arr) (x : nat) (path indexes : list nat) (v : val) : heap_arr :=
+	match path, indexes with
+		| nil, i::indexes     => h [(x, i) <- v]
+		| n::path, i::indexes => (arr_heap h n path indexes v) [(x, i) <- (varr n)]
+		| _, _                => empty val
+	end.
+
+Program Definition in_arr_aux (p : val) (path : list nat) (indexes : list val) (v : val) : asn :=
+	mk_asn (fun P k h => subheap (arr_heap (empty val) (val_to_arr p) path 
+                                               (List.map val_to_arr indexes) v) (snd h)) _ _ _.
+Next Obligation.
+	destruct h as [_h h]; destruct h' as [_h' h']; simpl in *.
+	apply subheap_prod in H as [_ H]; clear _h _h'.
+	rewrite H in H0. assumption.
+Qed.
+
+Definition in_arr (p : val) (indexes : list val) (v : val) : asn :=
+	Exists path : list nat, in_arr_aux p path indexes v.
+
+Fixpoint alloc_arr_val (h : heap_arr) (x size : nat) (f : nat -> val) : heap_arr :=
+	match size with
+		| 0   => h [(x, 0) <- (f x)]
+		| S n => (alloc_arr_val h x n f) [(x, S n) <- null]
+	end.
+
+Fixpoint alloc_arr_aux (h : heap_arr) (x : nat) (size : list nat) 
+         (paths : list (list nat)) : heap_arr :=
+	match size, paths with
+		| s::nil, nil            => alloc_arr_val h x s (fun x => null)
+		| s :: size, ps :: paths => List.fold_right (fun n h => h [(x, s) <- (varr n)]) h ps
+		| _, _                   => empty val
+	end.
+	
+Definition alloc_arr (x : nat) (size : list nat) (paths : list (list nat)) : heap_arr :=
+	alloc_arr_aux (empty val) x size paths.
+*)	
